translations/tsl_param3.v
@@ -1,19 +1,39 @@
 (* -*- coq-prog-args: ("-type-in-type" "-top" "Translations.tsl_param3") -*-  *)
 Require Import Template.All.
-From Translations Require Import translation_utils sigma.
+From Translations Require Import translation_utils.
 Import String Lists.List.ListNotations MonadNotation.
-Open Scope list_scope. Open Scope string_scope. Open Scope sigma_scope.
+Open Scope list_scope. Open Scope string_scope.
 
+Require Import MiniHoTT_paths.
 
 Reserved Notation "'tsl_ty_param'".
 
+
+Quote Definition tSigma := @sigT.
+Quote Definition tPair := @existT.
+Definition pair (typ1 typ2 t1 t2 : term) : term
+  := tApp tPair [ typ1 ; typ2 ; t1 ; t2].
+Definition pack (t u : term) : term
+  := tApp tSigma [ t ; u ].
+Definition sigma_ind := Eval compute in match tSigma with tInd i _ => i | _ =>  mkInd "bug: sigma not an inductive"%string 0 end.
+Definition proj1 (t : term) : term
+  := tProj (sigma_ind, 2, 0) t.
+Definition proj2 (t : term) : term
+  := tProj (sigma_ind, 2, S 0) t.
+Definition proj (b : bool) (t : term) : term
+  := tProj (sigma_ind, 2, if b then 0 else S 0) t.
+
+
 Fixpoint refresh_universes (t : term) {struct t} :=
   match t with
-  | tSort s => tSort []
+  | tSort s => tSort (if Universe.is_level s then s else [])
   | tProd na b t => tProd na b (refresh_universes t)
   | tLetIn na b t' t => tLetIn na b t' (refresh_universes t)
   | _ => t
   end.
+
+Local Instance tit : checker_flags
+  := {| check_univs := false |}.
 
 (* if b it is the first translation, else the second *)
 Fixpoint tsl_rec (fuel : nat) (Σ : global_context) (E : tsl_table) (Γ : context) (b : bool) (t : term) {struct fuel}
@@ -70,6 +90,7 @@ with tsl_term  (fuel : nat) (Σ : global_context) (E : tsl_table) (Γ : context)
   | S fuel =>
   match t with
   | tRel n => ret (tRel n)
+  | tSort s => ret (pair (tSort []) (tLambda (nNamed "A") (tSort []) (tProd nAnon (tRel 0) (tSort []))) (tSort s) (tLambda (nNamed "A") (tSort s) (tProd nAnon (tRel 0) (tSort s))))
   | tCast t c A => t' <- tsl_term fuel Σ E Γ t ;;
                   A' <- tsl_ty_param fuel Σ E Γ A ;;
                   ret (tCast t' c A')
@@ -90,11 +111,11 @@ with tsl_term  (fuel : nat) (Σ : global_context) (E : tsl_table) (Γ : context)
     end
   | t => match infer Σ Γ t with
          | Checked typ => let typ := refresh_universes typ in
-                          t1 <- tsl_rec fuel Σ E Γ true t ;;
-                        t2 <- tsl_rec fuel Σ E Γ false t ;;
-                        typ1 <- tsl_rec fuel Σ E Γ true typ ;;
-                        typ2 <- tsl_rec fuel Σ E Γ false typ ;;
-                        ret (pair typ1 typ2 t1 t2)
+                         t1 <- tsl_rec fuel Σ E Γ true t ;;
+                         t2 <- tsl_rec fuel Σ E Γ false t ;;
+                         typ1 <- tsl_rec fuel Σ E Γ true typ ;;
+                         typ2 <- tsl_rec fuel Σ E Γ false typ ;;
+                         ret (pair typ1 typ2 t1 t2)
         | TypeError t => raise (TypingError t)
         end
   end
@@ -113,17 +134,192 @@ Instance tsl_param : Translation
         tsl_ind := todo |}.
 
 
-Definition TslParam := @tTranslate tsl_param.
-Definition ImplParam := @tImplement tsl_param.
-
 
 Notation "'TYPE'" := (exists A, A -> Type).
-Notation "'El' A" := (sigma (π1 A) (π2 A)) (at level 20).
+Notation "'El' A" := (@sigT A.1 A.2) (at level 20).
+
+Run TemplateProgram (TC <- tImplement emptyTC "toto" (forall X, X) ;;
+                     tmPrint TC).
+Next Obligation.
+Abort.
+
 
 Definition Ty := Type.
-Set Printing Universes.
-Run TemplateProgram (TslParam emptyTC "Ty").
+(* Set Printing Universes. *)
+Run TemplateProgram (tTranslate emptyTC "Ty").
 Check Tyᵗ : El Tyᵗ.
+
+(* Definition mk_sig : forall {A} {B : A -> Type} (π1 : A), B π1 -> sigma A B *)
+(*   := @mk_sig. *)
+(* Axiom sigma_rect : forall A (B : A -> Type) (P : sigma A B -> Type), *)
+(*     (forall (x : A) (y : B x), P (mk_sig x y)) -> forall s, P s. *)
+(*   (* intros A B P X s. apply X. Defined. *) *)
+
+
+
+Run TemplateProgram (TC <- tImplementExisting emptyTC "sigT" ;;
+                     tmDefinition "TC" TC).
+Next Obligation.
+  unshelve econstructor.
+(*   - intros A B. refine (sigma (El A) (fun x => sigma (B.1 x) (B.2 x))). *)
+(*   - cbn. intros A B X. exact unit.  *)
+(* Defined. *)
+  - intros A B. refine (@sigT (El A) B.1).
+  - cbn; intros A B. refine (fun x => B.2 x.1 x.2).
+Defined.
+
+Run TemplateProgram (TC <- tImplementExisting TC "existT" ;;
+                     tmDefinition "TC'" TC).
+Next Obligation.
+  unshelve econstructor.
+(*   - intros A B x y. econstructor. exact y. *)
+(*   - intros A B π1 H. constructor.  *)
+(* Defined. *)
+  - intros A B x y. econstructor. exact y.1.
+  - cbn; intros A B x y. exact y.2.
+Defined.
+
+(* Compute TC'.  *)
+Time Run TemplateProgram (TC <- tImplementExisting TC' "sigT_ind" ;;
+                          tmDefinition "TC''" TC).
+Check "yo".
+Next Obligation.
+  unshelve econstructor.
+(*   - intros A B P [X1 X2] [s []]. apply X1. *)
+(*   - intros A B P [X1 X2] [s []]. apply X2. *)
+(* Defined. *)
+  - intros A B P [X1 X2] [s s']. apply (X1 s.1 (s.2; s')).
+  - intros A B P [X1 X2] [s s']. apply (X2 s.1 (s.2; s')).
+Defined.
+
+
+Run TemplateProgram (TC <- tImplementExisting TC'' "paths" ;;
+                     tmDefinition "TC3" TC).
+Next Obligation.
+  unshelve econstructor.
+  - intros A x y. refine (x.1 = y.1).
+  - cbn; intros A x y p. refine (p # x.2 = y.2).
+Defined.
+
+
+Run TemplateProgram (TC <- tImplementExisting TC3 "idpath" ;;
+                     tmDefinition "TC4" TC).
+Next Obligation.
+  unshelve econstructor; reflexivity.
+Defined.
+
+Run TemplateProgram (TC <- tImplementExisting TC4 "paths_ind" ;;
+                     tmDefinition "TC5" TC).
+Next Obligation.
+  unshelve econstructor.
+  - intros A [x x'] P X [y y'] [p q]. cbn in *. destruct p, q; cbn.
+    exact X.1.
+  - intros A [x x'] P X [y y'] [p q]. cbn in *. destruct p, q; cbn.
+    exact X.2.
+Defined.
+
+
+Definition Funext := forall A (B : A -> Type) (f g : forall x, B x), (forall x, paths (f x) (g x)) -> paths f g.
+
+Run TemplateProgram (tTranslate TC5 "Funext").
+
+Goal Funext -> El Funextᵗ.
+  simpl. intro H. unshelve econstructor.
+  - intros A B f g X. apply H. exact X.1.
+  - intros A B f g [X1 X2]; cbn in *.
+    apply H. intro x. rewrite transport_forall_constant.
+    specialize (X2 x).
+    refine (_ @ X2).
+    rewrite transport_compose.
+    eapply ap10. eapply ap.
+    rewrite ap_apply_lD.
+Admitted.
+
+
+Definition FALSE := forall X, X.
+Run TemplateProgram (tTranslate emptyTC "FALSE").
+
+Proposition consistency_preservation : El FALSEᵗ -> FALSE.
+  compute.
+  intros [f _] X.
+  exact (f (X; fun _ => unit)).
+Defined.
+
+
+Definition UIP := forall A (x y : A) (p q : paths x y), paths p q.
+
+Run TemplateProgram (tTranslate TC5 "UIP").
+
+Proposition uip_preservation : UIP -> El UIPᵗ.
+  simpl. intro H. unshelve econstructor.
+  - intros A x y p q. apply H.
+  - cbn. intros A x y p q.  apply H.
+Defined.
+
+Notation " A × B " := (@sigT A (fun _ => B)) (at level 30) : type_scope.
+
+Definition equiv (A B : Type) : Type :=
+  (* Type. *)
+  exists (f : A -> B) (g : B -> A),
+    (forall x, paths (g (f x)) x) × (forall x, paths (f (g x)) x).
+
+Run TemplateProgram (TC <- tImplementExisting TC5 "False" ;;
+                     tmDefinition "TC6" TC).
+Next Obligation.
+  unshelve econstructor.
+  - exact False.
+  - intros _. exact False.
+Defined.
+
+
+
+
+Check "go".
+Run TemplateProgram (
+                       ΣE <- tTranslate TC6 "equiv" ;;
+                       tmPrint "lo" ;;
+                       H <- tImplement ΣE "notUnivalence"
+                       (exists A B : Set, (equiv A B) × exists P, P A × ((P B) -> False)) ;;
+                       tmPrint "done"
+                     ).
+Check "proof".
+Next Obligation.
+Set Printing Universes. compute. unshelve econstructor. exists (bool:Type; fun _=> unit:Type).
+
+simple refine (existᶠ · _ · _ · _ · _).
+exact (bool:Type; fun _=> unit:Type).
+simple refine (existᶠ · _ · _ · _ · _).
+exact (unit:Type; fun _ => bool:Type).
+simple refine (existᶠ · _ · _ · _ · _).
+- simple refine (existᶠ · _ · _ · _ · _).
+  exists π2. exact π1.
+  simple refine (existᶠ · _ · _ · _ · _).
+  exists π2. exact π1.
+  simple refine (existᶠ · _ · _ · _ · _);
+    cbn; unshelve econstructor; reflexivity.
+- simple refine (existᶠ · _ · _ · _ · _).
+  exact HasTwoElFstComponentᵗ.
+  simple refine (existᶠ · _ · _ · _ · _).
+  + cbn. refine (_; tt). exists true. exists false.
+    discriminate 1.
+  + compute.
+    split; (intro p;
+            destruct p as [p _];
+            destruct p as [[] [[] p]];
+            contradiction p; reflexivity).
+Defined.
+
+Check "ok!".
+
+
+
+
+
+
+
+
+
+
 
 
 Definition mkTYPE (A₀ : Type) (Aᴿ : A₀ -> Type) : El Tyᵗ :=
@@ -155,18 +351,23 @@ unshelve refine (_ ; _).
 + refine (f.2 x).
 Defined.
 
-Notation "t · u" := (Appᶠ t u) (at level 65, left associativity).
+Notation "t · u" := (Appᶠ t u) (at level 64, left associativity).
 
 
 Definition sigmaᵀ (A : El Tyᵗ) (P : El (A →ᶠ Tyᵗ)) :=
   sigma (El A) (fun x => El (P · x)).
 
+Eval compute in sigmaᵀ.
 Definition existᵀ (A : El Tyᵗ) (P : El (A →ᶠ Tyᵗ))
            (x : El A) (y : El (P · x)) : sigmaᵀ A P
   := mk_sig x y.
 
 Inductive sigmaᴿ (A : El Tyᵗ) (P : El (A →ᶠ Tyᵗ)) : sigmaᵀ A P -> Type :=
 | existᴿ : forall (x : El A) (y : El (P · x)), sigmaᴿ A P (existᵀ A P x y).
+
+Goal forall (A : El Tyᵗ) (P : El (A →ᶠ Tyᵗ)) x, sigmaᴿ A P x.
+destruct x; constructor .
+Defined.
 
 Definition sigmaᶠ : El (Πᶠ (A : El Tyᵗ) (P : El (A →ᶠ Tyᵗ)), Tyᵗ).
 Proof.
@@ -181,22 +382,21 @@ refine (λᶠ A P x y, _).
 refine (mk_sig (existᵀ A P x y) (existᴿ A P x y)).
 Defined.
 
-Inductive eq@{i} {A : Type@{i}} (x : A) : A -> Type@{i} :=  eq_refl : eq x x.
 
-Inductive eq2 (A : El Tyᵗ) (x : El A) :
-  forall (y : El A), eq (π1 x) (π1 y) -> Prop :=
-| refl2 : eq2 A x x (eq_refl _).
+Inductive paths2 (A : El Tyᵗ) (x : El A) :
+  forall (y : El A), (π1 x) = (π1 y) -> Type :=
+| refl2 : paths2 A x x 1.
 
 
-Definition eqᶠ : El (Πᶠ (A : El Tyᵗ), A →ᶠ A →ᶠ Tyᵗ).
+Definition pathsᶠ : El (Πᶠ (A : El Tyᵗ), A →ᶠ A →ᶠ Tyᵗ).
 Proof.
 refine (λᶠ A x y, _).
 unshelve refine (mkTYPE _ _).
-+ refine (eq x.1 y.1).
-+ refine (eq2 A x y).
++ refine (paths x.1 y.1).
++ refine (paths2 A x y).
 Defined.
 
-Definition reflᶠ : El (Πᶠ (A : El Tyᵗ) (x : El A), eqᶠ · A · x · x).
+Definition reflᶠ : El (Πᶠ (A : El Tyᵗ) (x : El A), pathsᶠ · A · x · x).
 Proof.
 refine (λᶠ A x, _).
 unshelve refine (_; refl2 A x).
@@ -208,29 +408,29 @@ Defined.
   
 
 Quote Recursively Definition sigma_prog := @sigma.
-Quote Recursively Definition eq_prog := @eq.
+Quote Recursively Definition paths_prog := @paths.
 Quote Recursively Definition false_prog := @False.
 Definition sigma_decl := Eval compute in
       lookup_mind_decl "Translations.sigma.sigma" (fst sigma_prog).
-Definition eq_decl := Eval compute in
-      lookup_mind_decl "Translations.tsl_param3.eq" (fst eq_prog).
+Definition paths_decl := Eval compute in
+      lookup_mind_decl "Translations.MiniHoTT_paths.paths" (fst paths_prog).
 Definition false_decl := Eval compute in
       lookup_mind_decl "Coq.Init.Logic.False" (fst false_prog).
 
 
 Definition ΣE : option tsl_context :=
   sd <- sigma_decl ;;
-  ed <- eq_decl ;;
+  ed <- paths_decl ;;
   fd <- false_decl ;;
   let Σ' := [InductiveDecl "Coq.Init.Logic.False" fd;
-            InductiveDecl "Translations.tsl_param.eq" ed;
+            InductiveDecl "Translations.MiniHoTT_paths.paths" ed;
             InductiveDecl "Translations.sigma.sigma" sd] in
   let Σ' := reconstruct_global_context Σ' in
   let E' := [(IndRef (mkInd "Translations.sigma.sigma" 0),
               tConst "sigmaᶠ" []);
              (ConstructRef (mkInd "Translations.sigma.sigma" 0) 0,
               tConst "existᶠ" []);
-             (IndRef (mkInd "Translations.tsl_param.eq" 0), tConst "eqᶠ" []);
+             (IndRef (mkInd "Translations.MiniHoTT_paths.paths" 0), tConst "pathsᶠ" []);
              (IndRef (mkInd "Coq.Init.Logic.False" 0), tConst "Falseᶠ" [])
             ] in
   ret (Σ', E').
@@ -239,60 +439,3 @@ Definition HasTwoElFstComponentᵗ : El (Tyᵗ →ᶠ Tyᵗ)
   := λᶠ (T : El Tyᵗ), mkTYPE (exists (x y : T.1), x = y -> False) (fun _ => unit).
 
 
-Definition equiv (A B : Type) : Type :=
-  (* Type. *)
-  exists (f : A -> B) (g : B -> A),
-    (forall x, eq (g (f x)) x) × (forall x, eq (f (g x)) x).
-
-Definition FALSE := forall X, X.
-Run TemplateProgram (TslParam emptyTC "FALSE").
-
-Proposition consistency_preservation : El FALSEᵗ -> FALSE.
-  compute.
-  intros [f _] X.
-  exact (f (X; fun _ => unit)).
-Defined.
-
-Quote Definition equiv_ := Eval compute in equiv.
-
-
-Check "go".
-
-Fail Run TemplateProgram (match ΣE with
-                     | None => tmFail "bug: no tsl_ctx"
-                     | Some ΣE =>
-                       ΣE <- TslParam ΣE "equiv" ;;
-                       (* tmPrint ΣE' ;; *)
-                       tmPrint "lo" ;;
-                       H <- ImplParam ΣE "notUnivalence"
-                       (exists A B : Type, (equiv A B) × exists P, P A × ((P B) -> False)) ;;
-                       (* (exists A : Type, (equiv A A)) ;; *)
-                       tmPrint "done"
-                     end).
-Set Printing Universes.
-Check "proof".
-Next Obligation.
-simple refine (existᶠ · _ · _ · _ · _).
-exact (bool:Type; fun _=> unit:Type).
-simple refine (existᶠ · _ · _ · _ · _).
-exact (unit:Type; fun _ => bool:Type).
-simple refine (existᶠ · _ · _ · _ · _).
-- simple refine (existᶠ · _ · _ · _ · _).
-  exists π2. exact π1.
-  simple refine (existᶠ · _ · _ · _ · _).
-  exists π2. exact π1.
-  simple refine (existᶠ · _ · _ · _ · _);
-    cbn; unshelve econstructor; reflexivity.
-- simple refine (existᶠ · _ · _ · _ · _).
-  exact HasTwoElFstComponentᵗ.
-  simple refine (existᶠ · _ · _ · _ · _).
-  + cbn. refine (_; tt). exists true. exists false.
-    discriminate 1.
-  + compute.
-    split; (intro p;
-            destruct p as [p _];
-            destruct p as [[] [[] p]];
-            contradiction p; reflexivity).
-Defined.
-
-Check "ok!".
